heap_model_direct/SeparationLogic.v
@@ -1,0 +1,17 @@
+Require Import VST.msl.seplog.
+Require Import VST.msl.sepalg.
+Require Import VST.msl.alg_seplog_direct.
+Require Import RamifyCoq.msl_ext.abs_addr.
+Require Import RamifyCoq.msl_ext.seplog.
+Require Import RamifyCoq.msl_ext.alg_seplog_direct.
+Require Import RamifyCoq.heap_model_direct.SeparationAlgebra.
+Require Import RamifyCoq.heap_model_direct.mapsto.
+Require Import VST.msl.predicates_sa.
+
+Instance Ndirect : NatDed (pred world) := algNatDed world.
+Instance Sdirect : SepLog (pred world) := algSepLog world.
+Instance Cldirect : ClassicalSep (pred world) := algClassicalSep world.
+(* Instance CSLdirect : CorableSepLog (pred world) := algCorableSepLog world. *)
+Instance PSLdirect : PreciseSepLog (pred world) := algPreciseSepLog world.
+Instance OSLdirect : OverlapSepLog (pred world) := algOverlapSepLog world.
+Instance DSLdirect : DisjointedSepLog (pred world) := algDisjointedSepLog world.
